core/Destruct.v
@@ -1,0 +1,33 @@
+From Ssara.Core Require Import RegAlloc.
+From Ssara.Core Require Import RegClass.
+
+(* https://xavierleroy.org/publi/parallel-move.pdf *)
+
+From Ssara.Core Require Import RegPregInstance.
+Existing Instance reg_preg_instance.
+
+(*
+  The parallel move type is defined as a list of assignments of type src -> dst
+*)
+Definition pmove : Type := list (reg * reg).
+
+Inductive state : Type :=
+  | State (l1 : pmove) (l2 : pmove) (l3 : pmove)
+.
+
+(* 
+Function stepf (s : state) : state :=
+  match s with
+  | State nil nil _ => s
+  | State ((src, dst) :: xs) nil l =>
+    if preg_eqb src dst
+    then State tl nil l
+    else State tl ((src, dst) :: nil) l
+  | State t ((src, dst) :: b) l =>
+    match 
+. *)
+
+(* Definition phi_to_swaps (ps : list phi) (pred : block) : list inst :=
+  let l := get_lbl prev in
+  let ps := get_phis b in
+. *)
