core/Dict.v
@@ -4,36 +4,36 @@ From Stdlib Require Import ListSet.
 
 Section Dict.
 
-Class DictClass := {
-  key : Set;
-  value : Type;
-  default : value;
-  key_eq_dec : forall k k' : key, {k = k'} + {k <> k'};
-}.
-Context {dict_instance : DictClass}.
+  Class DictClass := {
+    key : Set;
+      value : Type;
+      default : value;
+      key_eq_dec : forall k k' : key, {k = k'} + {k <> k'};
+  }.
+  Context {dict_instance : DictClass}.
 
-Definition dict : Type := set key * (key -> value).
-Definition dict_empty : dict := (nil, fun _ => default).
+  Definition dict : Type := set key * (key -> value).
+  Definition dict_empty : dict := (nil, fun _ => default).
 
-Definition dict_update (d : dict) (k : key) (v : value) : dict :=
-  let (keys, m) := d in
-  (set_add key_eq_dec k keys, fun k' => if key_eq_dec k' k then v else m k')
-.
+  Definition dict_update (d : dict) (k : key) (v : value) : dict :=
+    let (keys, m) := d in
+    (set_add key_eq_dec k keys, fun k' => if key_eq_dec k' k then v else m k')
+  .
 
-Definition dict_map (d : dict) (k : key) : value :=
-  let (_, m) := d in m k
-.
+  Definition dict_map (d : dict) (k : key) : value :=
+    let (_, m) := d in m k
+  .
 
-Definition dict_keys (d : dict) : set key :=
-  let (keys, _) := d in keys
-.
+  Definition dict_keys (d : dict) : set key :=
+    let (keys, _) := d in keys
+  .
 
-Definition dict_values (d : dict) : set value :=
-  let (keys, m) := d in map m keys
-.
+  Definition dict_values (d : dict) : set value :=
+    let (keys, m) := d in map m keys
+  .
 
-Definition dict_list (d : dict) : list (key * value) :=
-  let (keys, m) := d in map (fun k => (k, m k)) keys
-.
+  Definition dict_list (d : dict) : list (key * value) :=
+    let (keys, m) := d in map (fun k => (k, m k)) keys
+  .
 
 End Dict.
