core/RegPregInstance.v
@@ -1,4 +1,5 @@
 From Stdlib Require Import PeanoNat.
+From Stdlib Require Import ListSet.
 From Ssara.Core Require Import RegClass.
 From Stdlib Require Import Lists.List.
 Import ListNotations.
@@ -52,3 +53,9 @@ Instance reg_preg_instance : RegClass := {|
   reg_eqb := preg_eqb;
   reg_eq_dec := preg_eq_dec;
 |}.
+
+Definition pregs_union := set_union reg_eq_dec.
+Definition pregs_diff := set_diff reg_eq_dec.
+Definition pregs_add := set_add reg_eq_dec.
+Definition pregs_remove := set_remove reg_eq_dec.
+Definition pregs_mem := set_mem reg_eq_dec.
