core/RegVregInstance.v
@@ -1,4 +1,5 @@
 From Stdlib Require Import PeanoNat.
+From Stdlib Require Import ListSet.
 From Ssara.Core Require Import RegClass.
 
 Definition vreg : Set := nat.
@@ -8,3 +9,10 @@ Instance reg_vreg_instance : RegClass := {|
   reg_eqb := Nat.eqb;
   reg_eq_dec := Nat.eq_dec;
 |}.
+
+(* Set of virtual registers *)
+Definition vregs_union := set_union reg_eq_dec.
+Definition vregs_diff := set_diff reg_eq_dec.
+Definition vregs_add := set_add reg_eq_dec.
+Definition vregs_remove := set_remove reg_eq_dec.
+Definition vregs_mem := set_mem reg_eq_dec.
