core/Utils.v
@@ -8,30 +8,10 @@ From Stdlib Require Import Lists.List.
 From Ssara.Core Require Import RegVregInstance.
 Existing Instance reg_vreg_instance.
 
-(* Set of virtual registers *)
-Definition vreg_eq_dec : forall r r' : reg, {r = r'} + {r <> r'} := reg_eq_dec.
-Definition vregs_union := set_union reg_eq_dec.
-Definition vregs_diff := set_diff reg_eq_dec.
-Definition vregs_add := set_add reg_eq_dec.
-Definition vregs_remove := set_remove reg_eq_dec.
-Definition vregs_mem := set_mem reg_eq_dec.
-
 (* Convert option to list *)
 Definition option_to_list {A : Type} (x : option A) : list A :=
   match x with
   | Some x' => x' :: nil
   | None => nil
-  end
-.
-
-(* Convert list option to list *)
-Fixpoint list_option_to_list {A : Type} (l : list (option A)) : list A :=
-  match l with
-  | nil => nil
-  | x :: xs =>
-    match x with
-    | Some y => y :: (list_option_to_list xs)
-    | None => (list_option_to_list xs)
-    end
   end
 .
